WIP

theories/Sim.v
@@ -5,6 +5,7 @@ Require Import Behavior.
 From Paco Require Import paco.
 Require Import RelationClasses List.
 Require Import ClassicalChoice PropExtensionality FunctionalExtensionality.
+Require Import Program.
 
 Set Implicit Arguments.
 
@@ -37,6 +38,42 @@ Definition single X (x: X): X -> Prop := fun x0 => x = x0.
 (*     _sim sim sss_src0 sss_tgt0 *)
 (* . *)
 
+Definition option_to_list X (ox: option X): list X := match ox with | Some x => [x] | _ => [] end.
+Coercion option_to_list_coercion := option_to_list.
+
+Inductive Star L (P: L.(state) -> Prop) (st0: L.(state)): (list event) -> (L.(state)) -> Prop :=
+| star_refl
+    (PROP: P st0)
+    (* ev_sum *)
+    (* (EV: ev_sum = []) *)
+  :
+    Star L P st0 [] st0
+| star_step
+    (PROP: P st0)
+    ev evs st1 st2
+    (STEP: L.(step) st0 ev st1)
+    (STAR: Star L P st1 evs st2)
+    (* ev_sum *)
+    (* (EV: ev_sum = ev ++ evs) *)
+  :
+    Star L P st0 (ev ++ evs) st2
+.
+
+Inductive Plus L (P: L.(state) -> Prop) (st0: L.(state)): (list event) -> (L.(state)) -> Prop :=
+| plus_intro
+    (PROP: P st0)
+    ev evs st1 st2
+    (STEP: L.(step) st0 ev st1)
+    (STAR: Star L P st1 evs st2)
+  :
+    Plus L P st0 (ev ++ evs) st2
+.
+
+Definition DPlus L (st0: (L.(state))) (evs: list event) (st1: L.(state)) :=
+  Plus L (fun st => L.(state_sort) st = demonic) st0 evs st1.
+Definition APlus L (st0: (L.(state))) (evs: list event) (st1: L.(state)) :=
+  Plus L (fun st => L.(state_sort) st = angelic) st0 evs st1.
+
 Lemma spin_nofinal
       L st0
       (SPIN: Beh.state_spin L st0)
@@ -47,6 +84,38 @@ Proof.
   punfold SPIN. inv SPIN; ii; rewrite H in *; ss.
 Qed.
 
+Lemma spin_noevent
+      L st0 e st1
+      (STAR: Star L (fun st => _.(state_sort) st = angelic) st0 [e] st1)
+      (SPIN: Beh.state_spin _ st0)
+  :
+    False
+.
+Proof.
+  remember [e] as tmp in STAR. revert Heqtmp.
+  induction STAR; ii; ss. punfold SPIN. inv SPIN; ii; rewrite PROP in *; ss.
+  destruct ev, evs; ss; clarify.
+  - exploit STEP0; eauto. i; des; ss.
+  - exploit STEP0; eauto. i; des; ss. pclearbot. eapply IHSTAR; eauto.
+Qed.
+
+Lemma spin_astar
+      L st0 st1
+      (STAR: Star L (fun st => _.(state_sort) st = angelic) st0 [] st1)
+      (SPIN: Beh.state_spin _ st0)
+  :
+    <<SPIN: Beh.state_spin _ st1>>
+.
+Proof.
+  remember [] as tmp in STAR. revert Heqtmp.
+  revert SPIN. induction STAR; ii; ss.
+  { destruct ev, evs; ss. dup SPIN. punfold SPIN. inv SPIN; rewrite PROP in *; ss.
+    exploit STEP0; eauto. i; des. pclearbot. eapply IHSTAR; ss.}
+Qed.
+
+
+
+
 Section SIM.
 
   Variable L0 L1: semantics.
@@ -55,68 +124,94 @@ Section SIM.
 
   Variant _sim sim (i0: idx) (st_src0: L0.(state)) (st_tgt0: L1.(state)): Prop :=
   | sim_final
-      (FINTGT: L1.(state_sort) st_tgt0 = final)
-      (FINSRC: L0.(state_sort) st_src0 = final)
+      (FINTGT: _.(state_sort) st_tgt0 = final)
+      (FINSRC: _.(state_sort) st_src0 = final)
     :
       _sim sim i0 st_src0 st_tgt0
-  | sim_demonic_tgt
-      (DEM: L1.(state_sort) st_tgt0 = demonic)
-      (DEMTGT: forall
-          st_tgt1
-          (STEPTGT: L1.(step) st_tgt0 None st_tgt1)
-        ,
-          exists i1, <<ORD: ord i1 i0>> /\ <<SIM: sim i1 st_src0 st_tgt1>>)
-    :
-      _sim sim i0 st_src0 st_tgt0
-  | sim_demonic_src
-      (DEM: L0.(state_sort) st_src0 = demonic)
-      (DEMSRC: exists
-          st_src1
-          (STEPSRC: L0.(step) st_src0 None st_src1)
-        ,
-          exists i1, <<ORD: ord i1 i0>> /\ <<SIM: sim i1 st_src1 st_tgt0>>)
-    :
-      _sim sim i0 st_src0 st_tgt0
-  | sim_demonic_both
-      (DEM: L0.(state_sort) st_src0 = demonic)
-      (DEM: L1.(state_sort) st_tgt0 = demonic)
-      (DEMTGT: forall
+  | sim_demonic
+      (DEM: _.(state_sort) st_tgt0 = demonic)
+      (STEPSIM: forall
           ev st_tgt1
-          (STEPTGT: L1.(step) st_tgt0 ev st_tgt1)
+          (STEPTGT: _.(step) st_tgt0 ev st_tgt1)
         ,
-          exists i1 st_src1, <<ORD: ord i1 i0>> /\ <<STEP: L0.(step) st_src0 ev st_src1>> /\
-                                                           <<SIM: sim i1 st_src0 st_tgt0>>)
+          exists i1 st_src1,
+            (<<PLUS: DPlus _ st_src0 ev st_src1>>
+             \/ (<<TAU: st_src1 = st_src0>> /\ <<TAU: ev = None>> /\ <<ORD: ord i1 i0>>))
+            /\
+            (<<SIM: sim i1 st_src1 st_tgt1>>))
     :
       _sim sim i0 st_src0 st_tgt0
-  | sim_angelic_src
-      (ANG: L0.(state_sort) st_src0 = angelic)
-      (ANGSRC: forall
-          st_src1
-          (STEPSRC: L0.(step) st_src0 None st_src1)
-        ,
-          exists i1, <<ORD: ord i1 i0>> /\ <<SIM: sim i1 st_src1 st_tgt0>>)
-    :
-      _sim sim i0 st_src0 st_tgt0
-  | sim_angelic_tgt
-      (ANG: L1.(state_sort) st_tgt0 = angelic)
-      (ANGTGT: exists
-          st_tgt1
-          (STEPTGT: L1.(step) st_tgt0 None st_tgt1)
-        ,
-          exists i1, <<ORD: ord i1 i0>> /\ <<SIM: sim i1 st_src0 st_tgt1>>)
-    :
-      _sim sim i0 st_src0 st_tgt0
-  | sim_angelic_both
-      (ANG: L0.(state_sort) st_src0 = angelic)
-      (ANG: L1.(state_sort) st_tgt0 = angelic)
-      (ANGSRC: forall
+  | sim_angelic
+      (ANG: _.(state_sort) st_src0 = angelic)
+      (STEPSIM: forall
           ev st_src1
-          (STEPSRC: L0.(step) st_src0 ev st_src1)
+          (STEPSRC: _.(step) st_src0 ev st_src1)
         ,
-          exists i1 st_tgt1, <<ORD: ord i1 i0>> /\ <<STEP: L1.(step) st_tgt0 ev st_tgt1>> /\
-                                                           <<SIM: sim i1 st_src0 st_tgt0>>)
+          exists i1 st_tgt1,
+            (<<PLUS: APlus _ st_tgt0 ev st_tgt1>>
+             \/ (<<TAU: st_tgt1 = st_tgt0>> /\ <<TAU: ev = None>> /\ <<ORD: ord i1 i0>>))
+            /\
+            (<<SIM: sim i1 st_src1 st_tgt1>>))
     :
       _sim sim i0 st_src0 st_tgt0
+  (* | sim_demonic_tgt *)
+  (*     (DEM: L1.(state_sort) st_tgt0 = demonic) *)
+  (*     (DEMTGT: forall *)
+  (*         st_tgt1 *)
+  (*         (STEPTGT: L1.(step) st_tgt0 None st_tgt1) *)
+  (*       , *)
+  (*         exists i1, <<ORD: ord i1 i0>> /\ <<SIM: sim i1 st_src0 st_tgt1>>) *)
+  (*   : *)
+  (*     _sim sim i0 st_src0 st_tgt0 *)
+  (* | sim_demonic_src *)
+  (*     (DEM: L0.(state_sort) st_src0 = demonic) *)
+  (*     (DEMSRC: exists *)
+  (*         st_src1 *)
+  (*         (STEPSRC: L0.(step) st_src0 None st_src1) *)
+  (*       , *)
+  (*         exists i1, <<ORD: ord i1 i0>> /\ <<SIM: sim i1 st_src1 st_tgt0>>) *)
+  (*   : *)
+  (*     _sim sim i0 st_src0 st_tgt0 *)
+  (* | sim_demonic_both *)
+  (*     (DEM: L0.(state_sort) st_src0 = demonic) *)
+  (*     (DEM: L1.(state_sort) st_tgt0 = demonic) *)
+  (*     (DEMTGT: forall *)
+  (*         ev st_tgt1 *)
+  (*         (STEPTGT: L1.(step) st_tgt0 ev st_tgt1) *)
+  (*       , *)
+  (*         exists i1 st_src1, <<ORD: ord i1 i0>> /\ <<STEP: L0.(step) st_src0 ev st_src1>> /\ *)
+  (*                                                          <<SIM: sim i1 st_src0 st_tgt0>>) *)
+  (*   : *)
+  (*     _sim sim i0 st_src0 st_tgt0 *)
+  (* | sim_angelic_src *)
+  (*     (ANG: L0.(state_sort) st_src0 = angelic) *)
+  (*     (ANGSRC: forall *)
+  (*         st_src1 *)
+  (*         (STEPSRC: L0.(step) st_src0 None st_src1) *)
+  (*       , *)
+  (*         exists i1, <<ORD: ord i1 i0>> /\ <<SIM: sim i1 st_src1 st_tgt0>>) *)
+  (*   : *)
+  (*     _sim sim i0 st_src0 st_tgt0 *)
+  (* | sim_angelic_tgt *)
+  (*     (ANG: L1.(state_sort) st_tgt0 = angelic) *)
+  (*     (ANGTGT: exists *)
+  (*         st_tgt1 *)
+  (*         (STEPTGT: L1.(step) st_tgt0 None st_tgt1) *)
+  (*       , *)
+  (*         exists i1, <<ORD: ord i1 i0>> /\ <<SIM: sim i1 st_src0 st_tgt1>>) *)
+  (*   : *)
+  (*     _sim sim i0 st_src0 st_tgt0 *)
+  (* | sim_angelic_both *)
+  (*     (ANG: L0.(state_sort) st_src0 = angelic) *)
+  (*     (ANG: L1.(state_sort) st_tgt0 = angelic) *)
+  (*     (ANGSRC: forall *)
+  (*         ev st_src1 *)
+  (*         (STEPSRC: L0.(step) st_src0 ev st_src1) *)
+  (*       , *)
+  (*         exists i1 st_tgt1, <<ORD: ord i1 i0>> /\ <<STEP: L1.(step) st_tgt0 ev st_tgt1>> /\ *)
+  (*                                                          <<SIM: sim i1 st_src0 st_tgt0>>) *)
+  (*   : *)
+  (*     _sim sim i0 st_src0 st_tgt0 *)
   .
 
   Definition sim: _ -> _ -> _ -> Prop := paco3 _sim bot3.
@@ -125,13 +220,16 @@ Section SIM.
   Proof.
     ii. inv IN; try (by econs; eauto).
 
-    - econs 2; et. ii. exploit DEMTGT; et. i; des; et.
-    - econs 3; et. des. esplits; eauto.
-    - econs 4; et. ii. exploit DEMTGT; et. i; des; et. esplits; et.
+    - econs 2; et. i. exploit STEPSIM; et. i; des; esplits; et.
+    - econs 3; et. i. exploit STEPSIM; et. i; des; esplits; et.
 
-    - econs 5; et. ii. exploit ANGSRC; et. i; des; et.
-    - econs 6; et. des. esplits; eauto.
-    - econs 7; et. ii. exploit ANGSRC; et. i; des; et. esplits; et.
+    (* - econs 2; et. ii. exploit DEMTGT; et. i; des; et. *)
+    (* - econs 3; et. des. esplits; eauto. *)
+    (* - econs 4; et. ii. exploit DEMTGT; et. i; des; et. esplits; et. *)
+
+    (* - econs 5; et. ii. exploit ANGSRC; et. i; des; et. *)
+    (* - econs 6; et. des. esplits; eauto. *)
+    (* - econs 7; et. ii. exploit ANGSRC; et. i; des; et. esplits; et. *)
   Qed.
 
   Hint Constructors _sim.
@@ -143,6 +241,56 @@ Section SIM.
     sim_init: exists i0, <<SIM: sim i0 L0.(initial_state) L1.(initial_state)>>;
   }
   .
+
+  Lemma adequacy_spin
+        (WF: well_founded ord)
+        i0 st_src0 st_tgt0
+        (SIM: sim i0 st_src0 st_tgt0)
+        (SPIN: Beh.state_spin L1 st_tgt0)
+    :
+      <<SPIN: Beh.state_spin L0 st_src0>>
+  .
+  Proof.
+    revert_until WF.
+    ginit.
+    { i. eapply cpn1_wcompat; eauto. eapply Beh.state_spin_mon. }
+    gcofix CIH. i.
+    revert_until i0. pattern i0. eapply well_founded_ind; eauto. clear i0. i.
+    rename x into i0. rename H into IH.
+
+    punfold SIM. inv SIM.
+    - eapply spin_nofinal in SPIN; ss.
+    - punfold SPIN. inv SPIN; rewrite DEM in *; ss. des. clarify.
+      rename st1 into st_tgt1.
+      exploit STEPSIM; eauto. pclearbot. i; des; rr in SIM; des; ss; cycle 1.
+      { clarify. eapply IH; eauto. }
+      inv PLUS. destruct ev, evs; ss. rename st_src1 into st_src2. rename st1 into st_src1.
+      clear - CIH STAR PROP STEP TL SIM.
+
+      gstep. econs 2; eauto. esplits; eauto. clear PROP STEP st_src0.
+      rename st_src1 into st_src0. rename st_src2 into st_src1.
+
+      remember [] as tmp in STAR. revert Heqtmp.
+      induction STAR; ii.
+      { gbase. eapply CIH; eauto. }
+      { rename st0 into st_src1. rename st1 into st_src2. rename st2 into st_src3.
+        destruct ev, evs; ss. gstep. econs 2; eauto. esplits; eauto. }
+    - gstep. econs; eauto. ii. exploit STEPSIM; eauto. i; des; ss; clarify; rr in SIM; des; ss; cycle 1.
+      { rename st1 into st_src1. esplits; eauto. exploit IH; eauto.
+        ii. eapply gpaco1_mon_gen; eauto. { eapply Beh.state_spin_mon. } ii; ss.
+      }
+      inv PLUS.
+      punfold SPIN. inv SPIN; ss; rewrite PROP in *; ss.
+      exploit STEP1; eauto. i; des. clarify. rr in TL; des; ss. clarify.
+      rename st_tgt1 into st_tgt2. rename st0 into st_tgt1. rename st1 into st_src1.
+
+      destruct ev; ss.
+      { exfalso. eapply spin_noevent; eauto. }
+      esplits; eauto.
+
+      gbase. eapply CIH; eauto.
+      eapply spin_astar; eauto.
+  Qed.
 
   Lemma adequacy_aux
         (WF: well_founded ord)
@@ -159,12 +307,59 @@ Section SIM.
     revert_until i0. pattern i0. eapply well_founded_ind; eauto. clear i0. i.
     rename x into i0. rename H into IH. rename x2 into tr.
 
+    destruct (classic (tr = Tr.spin)); clarify.
+    { punfold PR. inv PR; ss.
+      - exploit adequacy_spin; eauto. i. gstep. econs; eauto.
+      -
+    }
+
+    dup SIM.
     punfold SIM. inv SIM.
     - gstep. punfold PR. inv PR; ss; try rewrite FINTGT in *; clarify.
       + (** fin **) econs; ss; et.
       + (** spin **) eapply spin_nofinal in SPIN; ss.
+
     - punfold PR.
-      Require Import Program.
+      inv PR; ss; try rewrite DEM in *; clarify.
+      + (** spin **)
+        {
+          exploit CIH. eauto. pfold. econs 2; eauto. intro R.
+          punfold SPIN. inv SPIN; try rewrite DEM in *; ss. des. clarify. pclearbot.
+          rename st1 into st_tgt1.
+          exploit STEPSIM; eauto. i; des; r in SIM; des; ss; cycle 1.
+          { clarify. eapply IH; eauto. }
+          inv PLUS. rename st_src1 into st_src2. rename st1 into st_src1. destruct ev, evs; ss.
+          gstep. econs 5; eauto. rr. esplits; eauto.
+          exploit CIH. eauto. pfold. econs 2; eauto. intro RR.
+          inv STAR.
+          - econs.
+        }
+        punfold SPIN. inv SPIN; try rewrite DEM in *; ss. des. clarify. pclearbot.
+        rename st1 into st_tgt1.
+        exploit STEPSIM; eauto. i; des; r in SIM; des; ss; cycle 1.
+        { clarify. eapply IH; eauto. }
+        inv PLUS. rename st_src1 into st_src2. rename st1 into st_src1. destruct ev, evs; ss.
+        gstep. econs 5; eauto. rr. esplits; eauto.
+        inv STAR.
+        { econs; eauto. }
+      + (** nb **) gstep; econs; eauto.
+      + (** dem tau **)
+        rr in STEP. des. clarify.
+        exploit DEMTGT; et. i; des. r in SIM; des; ss. eapply IH; eauto.
+      + (** dem sys **)
+        rr in STEP. des. clarify. r in TL; des; ss.
+        exploit DEMTGT; et. i; des. r in SIM; des; ss.
+        rename st1 into st_tgt1.
+
+        gstep.
+        pfold.
+        (*** st_tgt0 --ev--> st_tgt1 ---> evs
+             st_src0
+         ***)
+        eapply IH; eauto. pfold. econs; eauto.
+        pfold. econs 6; eauto. eapply IH; eauto.
+
+    - punfold PR.
 
       inv PR; ss; try rewrite DEM in *; clarify.
       + (** spin **)
